Base: erasing gdim/bidx/bdim/tid

src/lib/kuiper/GPU.Base.fsti
@@ -27,28 +27,39 @@ let gpu : slprop = mode GPU
 val tid_t : Type0
 
 (* Arbitrary *)
-let max_blocks : erased int = 1024 * 1024
+let max_blocks : erased int = pow2 30
+
+let max_blocks_explicit : squash (reveal max_blocks == 1073741824) =
+  assert_norm (reveal max_blocks == 1073741824)
+
 (* Hard CUDA limit *)
 let max_threads : erased int = 1024
 
 (* Token for being in GPU block setup code *)
-val block_setup : (nthr: SZ.t { 0 < nthr /\ nthr <= max_threads }) -> slprop
+val block_setup (nthr: SZ.t { 0 < nthr /\ nthr <= max_threads })
+  : slprop
 
 (* Token for being a particular thread *)
-val thread_id : tid_t -> slprop
+val thread_id (tid : tid_t)
+  : slprop
 
 (* How many blocks total in the grid *)
-val gdim_x : tid_t -> (r:SZ.t { 0 < r /\ r <= max_blocks })
+val gdim_x (tid : tid_t)
+  : GTot (r:nat{0 < r /\ r <= max_blocks})
+
 (* Which block am I in? *)
-val bidx_x : (etid:tid_t) -> (r:SZ.t { r < gdim_x etid })
+val bidx_x (tid : tid_t)
+  : GTot (r:nat{r < gdim_x tid})
 
 (* How many threads per block *)
-val bdim_x : tid_t -> (r:SZ.t { 0 < r /\ r <= max_threads })
-(* Which thread am I in? *)
-val tidx_x : (etid:tid_t) -> (r:SZ.t { r < bdim_x etid })
-(* ^^ FIXME: Shouldn't all of these be Ghost, and returning a nat? *)
+val bdim_x (tid : tid_t)
+  : GTot (r:nat{0 < r /\ r <= max_threads})
 
-let thread_index (n: tid_t): GTot (i: nat { i < SZ.v (gdim_x n) * SZ.v (bdim_x n) }) = (
+(* Which thread am I in? *)
+val tidx_x (tid : tid_t)
+  : GTot (r:nat{r < bdim_x tid})
+
+let thread_index (n: tid_t): GTot (i: nat { i < gdim_x n * bdim_x n }) = (
   assert ((bidx_x n + 1) * bdim_x n <= gdim_x n * bdim_x n);
   bidx_x n * bdim_x n + tidx_x n
 )
@@ -57,31 +68,34 @@ let thread_count (n: tid_t): GTot pos = gdim_x n * bdim_x n
 fn block_idx_x () (#n: tid_t)
   requires thread_id n
   returns  id : U32.t
-  ensures  thread_id n ** pure (SZ.uint32_to_sizet id == bidx_x n)
+  ensures  thread_id n ** pure (U32.v id == bidx_x n)
 
 fn block_dim_x () (#n: tid_t)
   requires thread_id n
   returns  id : U32.t
-  ensures  thread_id n ** pure (SZ.uint32_to_sizet id == bdim_x n)
+  ensures  thread_id n ** pure (U32.v id == bdim_x n)
 
 fn thread_idx_x () (#n: tid_t)
   requires thread_id n
   returns  id : U32.t
-  ensures  thread_id n ** pure (SZ.uint32_to_sizet id == tidx_x n)
+  ensures  thread_id n ** pure (U32.v id == tidx_x n)
 
 let lemma_mul_lt (a b: nat) (c: nat { a < c }) (d: nat { b <= d /\ d > 0 }): Lemma (a * b < c * d) = ()
 
 noextract inline_for_extraction
 fn thread_idx_all () (#n: tid_t)
   requires thread_id n
-  returns  id : SZ.t
+  returns  id : SZ.t // FIXME: do we use SZ.t or U32.t for thread/block indices? Be consistent
   ensures  thread_id n ** pure (SZ.v id == thread_index n /\ SZ.v id < max_blocks * max_threads)
 {
-  assert (pure (bidx_x n < 1024 * 1024 /\ tidx_x n < 1024 /\ bdim_x n <= 1024));
-  lemma_mul_lt (SZ.v (bidx_x n)) (SZ.v (bdim_x n)) (1024 * 1024) 1024;
-  // assert (pure (bidx_x n * tidx_x n < 1024 * 1024 * 1024 /\ bdim_x n <= 1024));
+  assert (pure (bidx_x n < 1024 * 1024 * 1024 /\ tidx_x n < 1024 /\ bdim_x n <= 1024));
+  lemma_mul_lt (bidx_x n) (bdim_x n) (1024 * 1024 * 1024) 1024;
+  assert (pure (bidx_x n * tidx_x n < 1024 * 1024 * 1024 * 1024 /\ bdim_x n <= 1024));
   let bid = block_idx_x ();
   let bdim = block_dim_x ();
   let tid = thread_idx_x ();
-  SZ.add (SZ.mul (SZ.uint32_to_sizet bid) (SZ.uint32_to_sizet bdim)) (SZ.uint32_to_sizet tid) 
+  open FStar.SizeT;
+  let r =
+    (SZ.uint32_to_sizet bid *^ SZ.uint32_to_sizet bdim) +^ SZ.uint32_to_sizet tid;
+  r
 }
