src/examples/matmul-tile/GPU.MatMulTile.Kernel.fsti
@@ -97,15 +97,15 @@ fn kernel
   (* ^ 2nd and 3rd conjunct above just to help verifying this spec, sigh. *)
   (smem_sz : erased nat { smem_sz == 2 * SZ.v nthr })
   (ear: erased (gpu_array u64 smem_sz))
-  (etid : tid_t { gdim_x etid == nblk /\ bdim_x etid == nthr })
+  (etid : tid_t { gdim_x etid == SZ.v nblk /\ bdim_x etid == SZ.v nthr })
   requires gpu
     ** thread_id etid
     ** shmem_tok ear
-    ** Barrier.shared_pre nthr 0 ear (SZ.v (bidx_x etid)) (SZ.v (tidx_x etid))
+    ** Barrier.shared_pre nthr 0 ear (bidx_x etid) (tidx_x etid)
     ** kpre rows shared columns ga1 ga2 r #s1 #s2 (SZ.v nblk * SZ.v nthr)
          (tid_to_idx rows shared columns bdim (thread_index etid))
   ensures  gpu
     ** thread_id etid
-    ** Barrier.shared_pre nthr (2 * (shared / bdim)) ear (SZ.v (bidx_x etid)) (SZ.v (tidx_x etid))
+    ** Barrier.shared_pre nthr (2 * (shared / bdim)) ear (bidx_x etid) (tidx_x etid)
     ** kpost rows shared columns ga1 ga2 r #s1 #s2 (SZ.v nblk * SZ.v nthr)
          (tid_to_idx rows shared columns bdim (thread_index etid))
